>[!definition] Sum of Subspaces
>Let $\mathbf{V}$ we a vector space 
>let $W_{1},W_{2}\dots W_{n}$ be subspaces of $\mathbf{V}$
>The sum of theses subspaces denoted by $W_{1}+W_{2}+\dots +W_{n}$ is the space of all $v\in \mathbf{V}$ 
>$v=w_{1}+w_{2}+w_{3}+\dots+w_{n}; w_{i} \in W_{i} \ \forall \ i$
>Note: $W_{1}+W_{2}+\dots +W_{n}$ is a subspace of $\mathbf{V}$ 

>[!definition] Independence of Subspaces
>The subspace $W_{1},W_{2}\dots W_{n}$ is said to be independent if whenever
>$w_{1}+w_{2}+w_{3}+\dots w_{n}=0$ with $w_{i}\in W_{i}$ only if $w_{1}=w_{2}=w_{3}\dots=w_{n}=0$ 

>[!proposition]
>The sum of $W_{1},W_{2}\dots W_{n}$ is the smallest subspace containing all $W_{1},W_{2}\dots W_{n}$ i.e,
>if $E$ is subspace of $\mathbf{V}$ and $W_{i}\subseteq E, \forall \ i$ then $W_{1}+W_{2}+\dots W_{n} \subseteq E$

>[!definition] Direct sum
>$\mathbf{V}$ is said to be the direct sum of $W_{1},W_{2}\dots W_{n}$ if
>$\mathbf{V}=W_{1}+W_{2}\dots W_{n}$ and $W_{1},W_{2},W_{3}\dots W_{n}$ are independent
>we also represent direct sum by
>$\mathbf{V} = W_{1}\oplus W_{2} \oplus W_{3} \oplus \dots \oplus W_{n}$

>[!proposition]
>If $\mathbf{V}$ is the direct sum of $W_{1},W_{2}\dots W_{n}$ then
>$v\in \mathbf{V}$ can be written uniquely as the sum of $w_{i} \in W_{i}$ 

>[!proposition ] 
>let $W_{1},W_{2},W_{3}\dots W_{n}$ be subspace of a finite dimensional vector space $\mathbf{V}$, and let $\mathcal{B}_{i}$ be the basis for $W_{i}, \ \forall \ i\leq n$ 
>The order basis $\cal{B}$ obtained by listing the $\cal{B}_{1},\cal{B}_{2},\cal{B}_{3},\dots \cal{B}_{n}$ in order is a basis of $\mathbf{V}$ iff $\mathbf{V}=W_{1}\oplus W_{2}\oplus\dots\oplus W_{n}$ 

>[!corollary]
>Let $W$ be a subspace of $\mathbf{V}$. Then $\exists \ W'$ of $\mathbf{V}$ such that
>$$\mathbf{V}=W\oplus W'$$


`\begin{proof}`
let $u_{1},u_{2},u_{3},..u_{r}$ be a basis of $W$ extend this basis to $\mathbf{V}$ say $\left( u_{1},u_{2},u_{3}\dots u_{r},v_{1},v_{2},v_{3},\dots v_{n-r} \right)$
let $W'= \text{span}(v_{1},v_{2},v_{3},\dots v_{n-r})$ which is linearly independent so it is the basis ow $W'$ 
clearly, $W+W'=\mathbf{V}$ and $W$ and $W'$ are independent $\implies \mathbf{V} = W\oplus W'$ 
`\end{proof}` 
>[!definition] Compliment
> $W$' is called a complement of $W$ 

Note: Compliment is not unique

>[!prp ]
>Let $W_{2},W_{2}$ be sub-spaces of finite dimensional vector space $\mathbf{V}$ then,
>$$
>\dim(W_{1}+W_{2})=\dim W_{1}+ \dim W_{2}-\dim (W_{1}\cap W_{2})
>$$

`\begin{proof}`
let $r$ be the dimension of subspace $W_{1}\cap W_{2}$ and let $\left( u_{1},u_{2}\dots u_{r} \right)$ be the basis of it.
let basis of $W_{1}$ be $\left( u_{1},u_{2}\dots u_{r} ,v_{1},v_{2},\dots v_{n}\right)$ 
let basis of $W_{2}$ be $\left( u_{1},u_{2}\dots u_{r} ,w_{1},w_{2},\dots w_{n}\right)$ 
Claim: $\left( u_{1},u_{2}\dots u_{r} ,w_{1},w_{2},\dots w_{n},v_{1},v_{2},\dots v_{n}\right)$ is the basis of $W_{1}+W_{2}$ 
Clearly $\left( u_{1},u_{2}\dots u_{r} ,w_{1},w_{2},\dots w_{n},v_{1},v_{2},\dots v_{n}\right)$ spans $W_{1}+W_{2}$ 
lets show that $\left( u_{1},u_{2}\dots u_{r} ,w_{1},w_{2},\dots w_{n},v_{1},v_{2},\dots v_{n}\right)$ is independent
$$
\begin{align}
a_{1}u_{1}+\dots +a_{r}u_{r}+b_{1}v_{1}+\dots +b_{m-r}v_{m-r}+c_{1}w_{1}+\dots+c_{k-r}w_{k-r}=0
\end{align}
$$
$$
\begin{align} 
\underbrace{a_{1}u_{1}+\dots +a_{r}u_{r}}_{u}+\underbrace{b_{1}v_{1}+\dots +b_{m-r}v_{m-r}}_{x}=\underbrace{-c_{1}w_{1}-\dots-c_{k-r}w_{k-r}}_{y}
\end{align}
$$

^b488c5

$u+x \in W_{1}$ also $y\in W_{2}\implies x+u=y \in W_{1}\cap W_{2}$ 
As $y\in W_{1}\cap W_{2}\ \exists \ d_{i}$ such that
$$
y=d_{1}u_{1}+\dots d_{r}u_{r}
$$
$$
\begin{gather}
y-y & =0 \\
d_{1}u_{1}+\dots d_{r}u_{r}+c_{1}w_{1}+\dots+c_{k-r}w_{k-r} & =0
\end{gather}
$$
which implies $d_{i}=c_{i}=0 \ \forall \ i$ as $\left( u_{1},u_{2}\dots u_{r} ,w_{1},w_{2},\dots w_{n}\right)$ is the basis of $W_{2}\ \ \ \implies y=0$ 
so equation [[#^b488c5]] becomes
$$
\begin{align} 
\underbrace{a_{1}u_{1}+\dots +a_{r}u_{r}}_{u}+\underbrace{b_{1}v_{1}+\dots +b_{m-r}v_{m-r}}_{x}=0
\end{align}
$$
and as $\left( u_{1},u_{2}\dots u_{r} ,v_{1},v_{2},\dots v_{n}\right)$ is basis of $W_{1} \ \ a_{i}=b_{i}=0 \ \forall \ i$ 
`\end{proof}` 
#24-sep

> [!definition] 
> Let $W$ be a subset of $V$ and $U$ a compliment of $W$ in $V$ $i$,$e$. $V=W\oplus U$ 
> For $v\in V$ let $v=w+u$ where $w\in W, u\in U$
> $w$ is called the projection of $v\in V$ into $W$ along $U$ 

## Example 
let $(1,0)^{t}$ be the basis of $W$ and $\{ (1,0)^{t},(1,1)^{t} \}$ a basis of $V$ 

$$
\begin{align}
\begin{bmatrix}1 \\ 2\end{bmatrix}=c_{1}\begin{bmatrix}1 \\ 0\end{bmatrix}+c_{2}\begin{bmatrix}1 \\ 1\end{bmatrix}
\end{align}
$$
this is true if $c_{1}=-1,c_{2}=2$
$$
\begin{align}
\begin{bmatrix}1 \\ 2\end{bmatrix}=-1\begin{bmatrix}1 \\ 0\end{bmatrix}+2\begin{bmatrix}1 \\ 1\end{bmatrix} \\ \\

\begin{bmatrix}1 \\ 2\end{bmatrix}=\underbrace{ \begin{bmatrix}-1 \\ 0\end{bmatrix} }_{ w}+\underbrace{ \begin{bmatrix}2 \\ 2\end{bmatrix} }_{ u }
\end{align}
$$
> [!exercise] 
> Let $V=\mathbb{R}^{5}$
> $W=\{ (x_{1},x_{2},x_{3},x_{4},x_{5})^{t}:x_{1}+x_{4}=0\text{ and } 2x_{1}+x_{3}+x_{5}=0 \}$

let basis of $W$ be 
$$
\begin{align}
\left( v_{1}=\begin{bmatrix}-1\\0\\2\\1\\0\end{bmatrix},v_{1}=\begin{bmatrix}0\\1\\0\\0\\0\end{bmatrix} ,v_{3}=\begin{bmatrix}0\\0\\-1\\0\\1\end{bmatrix} \right) 
\end{align}
$$
we extend it to basis of $V$ by adding $e_{1},e_{4}$


> [!theorem] 
> Let $U$ be a complement of $W$ in $V$, ie $V=W\oplus U$ and define $P:V\implies V$ by $P(v)=w$ if $v=w+u$ for $w\in W,u\in U$ that is $P(v)$ is the projection of $v$ into $W$ along $U$ . $P$ is a linear transformation.
> this is called the projection operator into $W$ along $U$ 
> i) $P(v_{1}+v_{2})=P(v_{1})+P(v_{2}), \forall \ v_{1},v_{2}\in V$
> ii)$P(\alpha v)=\alpha P(v)$
> iii) if $v\in W,P(v)=P(v)$
> iv) if $v\in U,$ then $P(v)=0$
> v)$P^{2}=P$

 (todo::Prove you dumb ass) 

> [!exercise] 
> In the vector space $\mathbb{R}^{4}$ find two diffrent compliment of $W$ where $W$ is $\{ (x_{1},x_{2},x_{3},x_{4})^{t},x_{3}-x_{4}=0 \}$ 

first lets find the basis of W
$$
\begin{align}
\begin{bmatrix}
0 & 0 & 1 & 0 & -1
\end{bmatrix}X=0
\end{align}
$$
we assign arbitrary variable for non pivotal columns 

$x_3-x_{4}=0\implies x_{3}=x_{4}$
$X=\begin{bmatrix}x_{1}\\x_{2}\\x_{4}\\x_{4}\end{bmatrix}\implies X=x_{1}\begin{bmatrix}1\\0\\0\\0\end{bmatrix}+x_{2}\begin{bmatrix}0\\1\\0\\0\end{bmatrix}+x_{4}\begin{bmatrix}0\\0\\1\\1\end{bmatrix}$
Basis of $X$ is
$$
\begin{align}
\left\{ \begin{bmatrix}1\\0\\0\\0\end{bmatrix},\begin{bmatrix}0\\1\\0\\0\end{bmatrix},\begin{bmatrix}0\\0\\1\\1\end{bmatrix}\right\} 
\end{align}
$$
we can see that $e_{3}$ and $e_{4}$ are to different basis of compliment
 