#4-oct
>[!definition] Conditional Variance
> $$\var[X|Y=y] =\ex[{\left( X-\ex[X|Y=y] \right) |Y=y}] $$


> [!theorem] 
> $$\var[X]=\ex[{\var[X|Y] }] +\var[{\ex[X|Y] }] $$

`\begin{proof}`

 $$
\begin{align}
\var[X|Y] & =E[X^{2} +\left( \ex[X|Y] \right)^{2} -2X\ex[X|Y]|Y ] \\
 & =E[X^{2} |Y ] +E[ X |Y ]^{2}-2\ex[X|Y]^{2}  \\
 & =E[X^{2} |Y ] - & E[ X |Y ]^{2}  \\
\end{align}
$$

$$
\begin{align}
\ex[{\var[X|Y] }] & =\ex[X^{2} ] -\ex[{\ex[X|Y]^{2} }] \\

\end{align}
$$
$$
\begin{align}
\ex[{\var[X|Y] }] +\ex[{\ex[X|Y]^{2} }] -\ex[X] ^{2} & = \ex[X^{2} ] - \ex[X]^{2}  \\
 & = \var[X] 
\end{align}
$$
