
[[Probability/sheldon_ross.pdf#page=188&annotation=1215R|sheldon_ross, page 188]]

> [!definition] 
> Expectation of [[Probability/7. Continuous Random Variable|Continuous Random Variable]] 
> 
$$
\begin{align} \\
\ex[X]=\int^{+\infty }_{-\infty} xf_{X} (x)dx
\end{align}
$$

## Example
1. $X$ a RV with pdf
$$
\begin{align}
f(x) & = \begin{cases}
1, 0\leq x\leq1 \\
0, \text{other wise}
\end{cases}
\end{align}
$$

$$
\begin{align}
\ex[X]=\int^{-1}_{0}x 1 dx=\left[ \frac{a_{2}}{2} \right]  ^{1}_{0}   =\frac{1}{2} 
\end{align}
$$

If $Y=e^{ x }$

$$
\begin{align}
		F_{x} (y) & =0 \if Y<0 \\
			F_{Y}(y) & =P(e^{ X }\leq y)=P(X\leq \log y)   \\
 & =F_{x}(\ln y) 
\end{align}
$$
$$
\begin{align}
				f_{Y} (y)  & = \frac{d}{dy}F_{Y} (y) \\
		 & = \frac{1}{y}f_{X} (\ln y) \\
 & =\begin{cases}
 \frac{1}{y } \quad 1\leq y\leq e  \\
0
\end{cases}
\end{align}
$$
we can check 

$$
\begin{align}
		\int^{e}_{1} \frac{1}{y}dy & =1  
\end{align}
$$

Now the expectation 

$$
\begin{align}
				\ex[Y] & = \int^{e} _{1} y \frac{1}{y}dy \\
 & = e-1
\end{align}
$$

> [!lemma] 
> For non-negative RV The expected value of $Y$ is $\ex[Y]=\int_{0}^{\infty} P(Y>y)$ 


`\begin{proof}` 
Assume $Y$ has density $f_{y}$ 
$$
\begin{align}
\int^{\infty}_{0}P(Y>y)dy & =\int^{\infty}_{0}\left( \int^{\infty}_{y}f_{y}(z)dz    \right)     dy \\
 & = \int^{\infty}_{0} f_{y}(z)\left( \int^{z}_{0} dy   \right)dz    \\
 & = \int^{\infty}_{0}zf_{y}(z)dx  H  H\\
 & = \ex[Y] 
\end{align}
$$

 `\end{proof}`
 


> [!proposition]  [[Probability/sheldon_ross.pdf#page=189|prop 2.1]]
> $X$ be a RV pdf $f_{x}$ and let $g:\RR\to \RR$ then, 
> $$\ex[g(X)]=\int^{\infty}_{-\infty}g(x)f_{X}(x)dx$$


#15-Oct


`\begin{proof}` 
$$
\begin{align}
\ex[g(X)]  & =\int^{\infty}_{0} P(g(x)>y)   \\
 & =\int^{\infty }_{0}\int_{x:g(x)>y}   f_{x}(x)dxdy  \\
 & =  \int_{x:g(x)>0} \int^{g(x)}_{0}f_{x} (x)dydx  \\
 & = \int_{x:g(x)>0} g(x)f_{x}(x)dydx \\
 & = \int g(x)f_{x} (x)    \\
 
\end{align}
$$



 `\end{proof}`


[[Probability/sheldon_ross.pdf#page=190|Lemma 2.1]]

Using this to prove the previous example

$$
\begin{align}
\ex[e^{X} ] & =\int^{\infty} _{-\infty} e^{x} f_{x} (x)dx  \\
& = \int^{1} _{0} e^{x} dx \\
&  = e-1
\end{align}
$$
