# 1
$$
\begin{align}
E\left[ X \right]  & = \sum_{i=1}^{N}iP(X=i)\\
E\left[ X \right]  & = \sum_{i=1}^{N} \frac{i}{N}\\
E\left[ X \right]  & = \frac{1}{N}\sum_{i=1}^{N} {i}\\
E\left[ X \right]  & = \frac{1}{N} \cdot \frac{N*(N+1)}{2}\\
E\left[ X \right]  & =\frac{(N+1)}{2}\\
\end{align}
$$
$$
\begin{align}
E\left[ X ^{2}\right]  & = \sum_{i=1}^{N}i^{2}P(X=i)\\
E\left[ X ^{2}\right]  & = \sum_{i=1}^{N}i^{2} \frac{1}{N}\\
E\left[ X ^{2}\right]  & = \frac{1}{N}\cdot\sum_{i=1}^{N}i^{2} \\
E\left[ X ^{2}\right]  & = \frac{1}{N}\cdot \left( \frac{N(2N+1)(N+1)}{6} \right) \\
E\left[ X ^{2}\right]  & = \frac{(2N+1)(N+1)}{6}  \\
\end{align}
$$
$$
\begin{align}
\mathrm{Var} \left[ X \right]  & =\mathrm{E} \left[ X^{2}  \right] -(\mathrm{E} \left[ X \right] ) ^{2} \\
\mathrm{Var} \left[ X \right]  & = \frac{(2N+1)(N+1)}{6} -\left[\frac{(N+1)}{2}\right]^{2} \\
\mathrm{Var} \left[ X \right]  & = \frac{2(2N+1)(N+1)-3(N+1)^{2}}{12} \\
\mathrm{Var} \left[ X \right]  & = \frac{2\left(2N^{2} +3N+1\right)-3\left(N^{2} +2N+1\right)}{12} \\
\mathrm{Var} \left[ X \right]  & = \frac{N^{2} +0-1}{12} \\
\mathrm{Var} \left[ X \right]  & = \frac{N^{2} +0-1}{12} \\
\mathrm{Var} \left[ X \right]  & = \frac{N^{2} -1}{12} \\
\end{align}
$$
$\therefore$ The Variance of first $N$ natural numbers is $\frac{N^{2} -1}{12}$ 


# 2 
