
Suppose $a_{1},a_{2}\dots$ are real numbers 
$$\sum^{n}_{j=1}a_{j}=a_{1}+a_{2}\dots+ a_{n}$$
what is $\sum^{\infty}_{j=1}a_{j}=?$
for $a_{1},a_{2},\dots$ 
let $s_{n} = \sum^{n}_{j=1}a_{j}$ for $n\geq l$ then $s_{n}$ is called the partial sum 
that is 
$$
\begin{align}
s_{1} & =a_{1} \\
s_{2} & =a_{1}+a_{2} \\
\vdots \\ 
s_{n} & =a_{1}+a_{2}\dots a_{n} \\
\vdots 
\end{align}
$$
>[!definition ]  
>suppose $\left\{ a_{n} \right\}_{n\in \mathbb{N}}$ is a sequence of real numbers 
>Then the series $\sum^{\infty}_{j=1}a_{j}$ is said to converge if the sequence of partial sums $\left\{ s_{n} \right\}_{n\in \mathbb{N}}$ converges 
>that is $$\sum^{\infty}_{j=1}a_{j}=\lim_{ n \to \infty } s_{n}$$

If the series doesn't converge It is meaningless
## Examples
$$
a_{j}=
\begin{cases}
j \ \forall \ 1\leq j\leq_{1}0 \\
0,j>10
\end{cases}
$$
$$
\begin{align}
s_{1} & =1 \\
s_{2} & =1+2 \\
\vdots \\
s_{10} & =1+2+\dots 10 \\ 
s_{n} & =s_{10} \ \  \forall \ n\geq 10
\end{align}
$$
Here $s_{n}$ converges therefore so is the series.

A series converges if and only if there exist an $x \in\mathbb{R}$ such that for every $\epsilon>0$, there exist $k\in \mathbb{N}$ such that 
$$
	\left| \sum^{n}_{i=1}a_{j}-x \right| <\epsilon \ \ \ \forall \ n\geq k
$$

In terms of [[1. Cauchy Criterion#^5cfca9]] 

A series converges if and only if for every $\epsilon>0$ there exist $k\in \mathbb{N}$ such that
$$
\left| s_{n}-s_{m} \right| <\epsilon \ \ \ \forall \ k\leq m\leq n
$$
$$

\implies\left| \sum^{n}_{j=m} a_{j} \right| <\epsilon \ \ \ \forall \ k\leq m\leq n
$$

>[!theorem ] 
>For $x \in \mathbb{R}$ with $|x|<1$ 
>$$\sum^{\infty}_{n=0}x^{n}=\frac{1}{1-x}$$

`\begin{proof}`
For $n\in \mathbb{N}\cup \left\{ 0 \right\}$ 
$s_n=1+x^{1}+x^{2}+x^{3}+\dots +x^{n}=\frac{1-x^{n+1}}{1-x}$ 
$$
\lim_{ n \to \infty } s_{n}=\lim_{ n \to \infty } \frac{1-x^{n+1}}{1-x}= \lim_{ n \to \infty } \left(  \frac{1}{1-x} -\frac{x^{n+1}}{1-x}\right) =\frac{1}{1-x}
$$
using [Bernoulli's inequality](https://en.wikipedia.org/wiki/Bernoulli%27s_inequality) we can show $\lim_{ n \to \infty }x^{n}=0$ for $|x|<1$ 

`\end{proof}`

>[!theorem ]
>Suppose $\sum^{\infty}_{j=1}a_{j}$ is a convergent series of $\mathbb{R}$.
>Then $\lim_{ n \to \infty }a_{n}=0$

`\begin{proof}`
$$
a_{n}=s_{n}-s_{n-1} \ \ \ \forall \ n\geq{2}
$$
using [[1. Cauchy Criterion]] for $\epsilon>0\  \exists \ k\in \mathbb{N}$ such that
$$

\left| \sum^{n}_{j=m} a_{j} \right| <\epsilon \ \ \ \forall \ k\leq m\leq n
$$
let $n=m+1$ 
$$

\implies\left| \sum^{m+1}_{j=m} a_{j} \right| <\epsilon \
$$
$$

\implies\left| a_{m} \right| <\epsilon \
$$

`\end{proof}`
Note the converse is not true example $s_{n}=1+\frac{1}{2}+\frac{1}{3}\dots \frac{1}{n}$ does not converge we can show that $s_{n}$ converges to infinite

>[!theorem ] 
>let $\left\{ a_{n} \right\}_{n\in \mathbb{N}}$ be sequence of $\mathbb{R}^{+}$ 
>such that $\lim_{ n \to \infty }a_{n}=0$ and $a_{n}\geq a_{n+1} \forall\ n$ then
>$$\sum^{\infty}_{n=1}(-1)^{n+1}a_{n}\text{   is     convergent }$$

`\begin{proof}`
$$
s_{n}=\sum^{n}_{k=1}(-1)^{k-1}a_{k}
$$
$$
\begin{align}
s_{1} & =a_{1} \\
s_{2} & =a_{1}-a_{2} \\
	0\leq & s_{2}\leq s_{1} \\
s_{3} & =a_{1}-a_{2}+a_{3}=a_{1}-(a_{2}-a_{3}) \leq s_{1} \\

\end{align}
$$

>[!Claim ] 
$$\begin{gather} s_{2}\leq s_{4}\leq s_{6}\dots s_{2n} \forall \ n\\ s_{1}\geq s_{3}\geq s_{5}\geq \dots s_{2n+1} \forall \ n\end{gather}$$

To prove Both converge to same value (question::Hope Sir proves this )
