#15-oct
> [!def] 
> $f$ is said to be differentiable at $c$ if 
> 			$$\lim_{ x \to c } f_{c}(x) =\lim_{ x \to c } \frac{f(x)-f(c)}{x-c}$$
> 	then we write $f'(c)=\lim_{ x \to c }\frac{(f(x)-f(c))}{x-c}$ 

#16-oct 

let $I \subseteq \RR \st I\neq \phi$ and $I$ is not a single ton 

> [!definition] 
> Let $f:I\to \RR$ be a function suppose $c\in I$ then $f$ is said to be differentiable at $c$ if  $\lim_{ x \to c } \frac{f(x)-f(c)}{x-c}$ exist then $f'(c)=\lim_{ n \to \infty } \frac{f(x)-f(c)}{x-c}$


> [!theorem] 
> Suppose $f:I\to \RR$ is differentiable at $c$ $\in I$  then $f$ is continuous at $c$ converse is not true

`\begin{proof}` 
$$
\begin{align}
				\lim_{ x \to c } f(x)-f(c) & = \lim_{ x \to c } \frac{f(x)-f(c)}{c-x}(c-x) \\
				\lim_{ x \to c } f(x)-f(c) & = \lim_{ x \to c } \frac{f(x)-f(c)}{c-x}0\\
				\lim_{ x \to c } f(x)-f(c) & = 0 \\
		\implies 			\lim_{ x \to c } f(x) & = f(c) \\


\end{align}
$$

 `\end{proof}`


## Example 

1. Consider $f:[0,2]\to \RR \ \ f(x)=x^{3}$ 
take $c=1$ 

$$
\begin{align}
		\lim_{ x \to 1 } \frac{f(x)-f(c)}{x-c}  & =\lim_{ x \to 1 } \frac{x^{3} -1}{x-1} \\
	 & =\lim_{ x \to 1 } x-1 \frac{x^{2} +x+1}{x-1} \\
 & = 3 \\
\so f'(1) \exists \And =3
\end{align}
$$

> [!theorem] 
> suppose  $f,g:I\to \RR$ are functions differentiable at $c\in I$  then
> 1. $af+bg$ is differentiable at $c$ for $a,b,\in \RR$  and $(af+bg)'(c)=af'(c)+bf'(c)$
> 2. $fg$ is differentiable at $c$ and $fg(c)=f'(c)g(c)+g(c)f'(c)$


`\begin{proof}` 

1. 
$$
\begin{align}
				\lim_{ x \to c } \frac{(af+bg)(x)-(af+bg )(c)}{x-c} & =\lim_{ x \to c } \left[ \frac{a(f(x)-f(c))}{x-c} + b \frac{g(x)-g(c)}{x-c} \right]  \\
 & =af'(c)-bg'(c)
\end{align}
$$
2.
$$
\begin{align}
			\lim_{ x \to c } \frac{(fg)(x)-fg(c)}{x-c} & = \lim_{ x \to c } \frac{(fg)(x)-f(c)g(x)+f(c)g(x)-fg(c)}{x-c}  \\
& = \lim_{ x \to c } \frac{\left\{ (fg)(x)-f(c)g(x) \right\}+\left\{ f(c)g(x)-fg(c) \right\}}{x-c}  \\
		 & =\lim_{ x \to c } f'(c)g(c)+g'(c)f(c)
\end{align}
$$


 `\end{proof}`


> [!theorem] 
> Suppose $f,g:I\to \RR$ are functions diffrentiatable ar $c$ $\in I$ 
> if $g(c)\neq 0$ then $g(x)\neq0$ is same interval I containing $c$ on I $\frac{f}{g}$ is well defined and diffrentiable at $c$ 
> with
> $$\frac{f}{g}(c)= \frac{f'(c)g(c)-f(c)g(c)}{g(c)^{2} }$$

`\begin{proof}`  
As $g$ is diffrentiatable at $c$ it is continuous at $c$ 

takr $\upvarepsilon= \Mod[\frac{g(x)}{c}]$ as $g(c)\neq0$ we have $\upvarepsilon>0$
so $\exists \ \delta>0 \st$ 

$$
\begin{align}
\Mod[g(X)-g(1)]<\upvarepsilon \forall x \in(c-\delta,c+\delta) 
\end{align}
$$
so $g(x)\neq0$ for $x \in(c-\delta,c+\delta)$

take $J=(c-\delta,c+\delta)$


$$
\begin{align}
				\lim_{ x \to c } \frac{\left( \frac{f}{g}(c)-\frac{f}{g}(x) \right)}{c-x} & =\lim_{  x \to c }  \frac{1}{x-c} \left[ \frac{f(x)}{g(x)}-\frac{f(c)}{g(c)} \right] \\
				& =\lim_{  x \to c }  \frac{1}{x-c} \left[ \frac{g(c)f(x)-g(x)f(c)}{g(c)g(x)} \right] \\
				& =\lim_{  x \to c }  \frac{1}{g(c)g(x)} \left[ \frac{g(c)[f(x)-f(c)]- f(c)[g(x)-g(c)]}{x-c} \right] \\
				& =\frac{f'(c)g(c)-f(c)g(c)}{g(c)^{2} }\\
\end{align}
$$
 `\end{proof}`

> [!cor] 
> Suppose $p:\RR\to \RR$ is a real polynomial 
> $p(x)=a_{o}+a_{1}x+a_{2}x^{2}\dots a_{n}x^{n}, \forall \ x \in \RR$
> then at any $c \in \RR$ $p$ is differentiable at $c$ and 
> 
$p'(x)=a_{1}+a_{2}c+a_{3}c^{2}+\dots na_{n}c^{n-1}$
> 




> [!definition] 
> Let $f:I\to \RR$  be a function 
> 1.  $f$ said to be differentiable it is differentiable at every $c\in I$   
> $f'$ is a function on I called the first Derivative of f
> 2. if $f'$ is differentiable at every $c\in I$ then $f$ is said to be twice differentiable and $f'' \or f^{(2)}$ is a function  on I defined by $f''(c)=(f')'(c)$
> 3. for $n\in \NN \ \  n\geq1$ $f^{(n-1)}$ is differentiable at every $c\in I$ then $f$ is said to be $n$ times differentiable   
> $f^{(n)}={f^{(n-1)}}'(c)$ 
> 4. $f$ is said to be infinite differentiable if $f$ is n-times differentiable for every $n\in \NN$
> 5. $f$ is said to be continuously differentiable if $f$ is differentiable and  is continuous


> [!theorem] (chain rule)
> suppose $f:I\to R$ and $g:J\to R$ are function such that $f(I)\subseteq J$ take $h=gof$ suppose $f $
> 