
>[!lemma] 
>If $m$ and $n$ are each the sum of two squares then so is there product $mn$

`\begin{proof}`
$\left( a ^{2}+b^{2} \right)\left( c^{2}+d^{2} \right)=(ac + bd)^{2} + (ad-bc)^{2}$
`\end{proof}`
>[!theorem]
>A prime $p$ of form $4k+3$ can not be written as a sum of two squares

^8e7812

`\begin{proof}`
$$
\begin{align}
a ^{2} & =1,0 \pmod{4} \\
b^{2} & =1,0 \pmod{4} & \\
\implies a^{2}+b^{2} & =1,0,2 \pmod{4}
\end{align}
$$
`\end{proof}`

>[!lemma]
>let $p$ be a prime and let $\gcd(a,p)=1$ 
>The the congruenc
>$ax\equiv y \pmod{p}$
>admits a solution $x_{o},y_{o}$ where 
>$o<|x_{o}|<\sqrt{ p }$ and $a<|y_{o}|<\sqrt{ p }$

`\begin{proof}`
$k=\left[ \sqrt{ p } \right]+1$
consider the set
$S=\left\{ (x,y)|o\leq x\leq k-1,0\leq y\leq k-1 \right\}$
Note that $|S|=k^{2}>p$
[[1. Pigeonhole Principle#^6b5eb7]] implies that
$\exists \ x_{1},x_{2},y_{1},y_{2} \in \left\{ 0,1,2\dots k-1 \right\}$ where $x_{1} \not= x_{2}$ or $y_{1}\neq y_{2}$ such that
$$
ax_{1}-y\equiv ax_{2}-y_{2} \pmod{p}
$$
take,
$$
\begin{align}
x_{o} & =x_{1}-x_{2}\\
y_{o} & =y_{1}-y_{2} \\
\end{align}
$$
Note: 
$$
\begin{align}


x_{o},y_{o}  & \leq k-1  \\
\implies x_{o},y_{o} & <k \\
\implies x_{o},y_{o} & < \lfloor\sqrt{p} \rfloor+1 \\
\implies x_{o},y_{o} & <\sqrt{p} \\
\end{align}
$$

`\end{proof}`


>[!theorem]
>An odd prime $p$ is expressed as a sum of two squares iff 
>$p=1\pmod{4}$

`\begin{proof}`


“only if” part is done [[2. Sum of Two Squares#^8e7812]] 
let $p\equiv 1 \pmod{4}$ There exists an integer a such that 
$$
a ^{2} \equiv -1 \pmod{p}
$$
$$
\implies a^{2}k+1=p
$$
(question:: Please help me again) 
In fact, we can take $a=r^{\frac{p-1}{4}}$ where $r$ is the primitives root of $p$ 
Note that $\gcd(a,p)=1$ 
`\end{proof}`

>[!corollary] Uniqueness of $a,b$ such that $p=a^{2}+b^{2}$

`\begin{proof}`
$p=a^{2}+b ^{2}=c^{2}+d^{2}$
$$
\begin{align}
a^{2} & =p-b^{2} \\
d^{2} & =p-c^{2} \\
a^{2}d^{2} & =p^{2}-(b^{2}+c^{2})p +b^{2}c^{2} \\
a^{2}d^{2}-b^{2}c^{2} & =p^{2}-(b^{2}+c^{2})p  \\
\implies a^{2}b^{2}-b^{2}c^{2} & \equiv 0 \pmod{p}
\end{align}
$$
$\implies (ad-bc)(ad+bc)=0 \pmod{p}$
$p^{2}=(a^{2}+b^{2})(c^{2}+d^{2})=(ad+dc)^{2}+(ac-bd)^{2}$
lets assume W.L.O.G $p|ad+bc$ 
$$
\begin{align}
\end{align}
$$
Then
$$
\begin{align} \\
ac-bd & =0 \\
\implies ac & =bd \\
a & |bd  \\
\implies d & =ka \text{ since } gcd(a,b)=1 \\
ac & =bka\\
\implies c & =bk  \\
\text{ since } \gcd (c,d)=1 & \implies \gcd(c,k)=1 \\
\implies c & =b \text{ and } k=1
\end{align}
$$
similarly we can show $a=d$ 

if we chose $p|ad-bc$ then we get $a=c$ and $b=d$ 

hence They are unique
`\end{proof}`



>[!theorem]  
>let the positive integers n be written as $n=N^{2}m$ where $m$ is square-free. Then $n$ can be represented as the sum of two squares if and only if $m$ contains no prime factor of the form $4k+3$

`\begin{proof}`
Suppose $n=N^{2}m$ where $m$ has no prime factor of the form $4k+3$ if $m=1$ then $n=N^{2}+0^{2}$ done.
Let $m>1$ write $m=p_{1}p_{2}\dots p_{r}$ .
Each of the prime $p_{i}$, being of the form $4k+1$, can be written as the sum of squares,
which implies there product $m$ also can be written as $m=x^{2}+y^{2}$.
$$
\begin{align}
	n & =N^{2}m  \\
 & =N^{2}(x^{2}+{y^{2}}) \\
 & =(Nx)^{2}+(Ny)^2 \\
\end{align}
$$
The other way.
Suppose,
$n=a^2+b^{2}=N^{2}m$ 
assume that $m>1$ and let $p$ be an odd prime divisor of $m$ 
let $d=\gcd(a,b)$ then 
$a=rd$ and $b=sd$ where $\gcd(r,s)=1$
This gives $(r^{2}+s^{2})d^{2}=N^{2}m$ 
since $m$ is square-free we have $d|N$ 
$r^{2}+s^{2}\equiv \frac{N^{2}}{d^{2}}m\implies r^{2}+s^{2}\equiv0\pmod{p}$
since $(r,s)=1$ , $p$ cannot divide both $s$ and $r$ 
$\gcd(s,p)=\gcd (r,p)=1$
we can find $r'$ such that $r'r\equiv 1 \pmod{p}$
$$
\begin{align}
(r'r)^{2}+(r's)^{2} & =0\pmod{p} \\
\implies(r's)^{2} & =-1\pmod{p} \\
\end{align}
$$
$\implies -1\text{ is a quadratic residue }$
$\implies p\equiv {1}\pmod{4}$

