#20-sep 
## Quadratic Forms
> [!definition ]  Binary Quadratic Form
> A binary quadratic form (bqf) is a polynomial of the form 
> $q(x,y)=ax^{2}+bxy+xy^{2}$ with $a,bac\in \mathbb{Z}$ 
> we may think of it as a function
> $q:\mathbb{Z}^{2}\to \mathbb{Z}$
> $(x,y)\to ax^{2}+bxy+xy^{2}$ 
> In short we write $q=(a,b,c)$ 

^ebdd1f

We say that $q=(a,b,c)$ is a primitive if $gcd(a,b,c)=1$
We say that $q$ represents the integer $n\in \mathbb{Z}=n$ for some $x,y\in \mathbb{Z}, (x,y)\neq(0,0)$  
We it represent primitively or properly if $n=q(x,y)$ and $\gcd(x,y)=1$ 

> [!remark ] 
> The same number can be represented primitively and non primitively

> [!definition ]  Disc of Binary Quadratic Form
> for $q=(a,b,c)$ we define 
$$
\text{disc}(q)=b^{2}-4ac
$$


>[!prp ]   
>Let $q=(a,b,c)$ be a [Binary Quadratic Form](#^ebdd1f) with $\text{disk}(q)=D=b^{2}-4ac$
>i) then $q$ represent 0 $\iff$ $D$ is a square 
>ii) $D\leq0\iff$ all non zero values represented by $q$ are of the same sign


`\begin{proof}`
Case I: $a=0$ then
$$
q(x,y)=bxy+cy^{2} \implies D=b^{2}-4ac=b^{2}
$$
also 
$$
q(x,0)=0 \ \forall \ x \in \mathbb{Z}
$$
this proves i) for this case
for ii) $D\leq{0}\iff b^{2}\leq{0}\iff b=0$ 
then $q(x,y)=cy^{2}$ 
This shows that all values of $q$ has the same sign of $c$ 
Case II: $a\neq 0$ then,
$$
\begin{align}
4aq(x,y) & =4a^{2}x^{2}+4abxy+4acy^{2} \\
 & =\left\{  (2ax)^{2}+2(2ax)(by)+(by)^{2}\right\} -(by)^{2} +4acy^{2} \\
 & =\left\{  (2ax)^{2}+2(2ax)(by)+(by)^{2}\right\} -y^{2}\left( b^{2}-4ac \right) \\
 & =\left( 2ax+by \right) ^{2} -y^{2}D \\
\end{align}
$$

$$
\implies4aq(x,y)=(2ax+by)^{2}-D^{}y^{2}
$$

^6d9892

Clearly, $0$ is represented (question::For what value?) 
let $(x,y)=(\sqrt{ D }-b,2a)$ 
$$
\iff \exists \ (x,y)\in \mathbb{Z}^{2} \setminus \left\{ (0,0) \right\} 
$$
such that
$$
(2ax+by)^{2}=Dy^{2} 
$$
which implies $D$ is a square.(question::we have shown if it represents 0 then its d is square how to show the other way)
This proves i)
for ii) if $D\leq{0}$ then clearly 
$4aq(x,y)\geq{0} \ \forall\ x,y$ so $q(x,y)$ is of constant sign( same as $a$) from [[#^6d9892]]
conversely suppose $q(x,y)$ is of constant sign then
$$
4aq(-b,2a)=-4a^{2}D
$$
and 
$$
4aq(1,0)=4a^{2}
$$
are of the same sign (by hypothesis), so
$$
\begin{align}
\text{as } 4a^{2} & \geq0 \\
\implies -4a^{2}D & \geq0 \\
\implies D & \leq0

\end{align}
$$
> [!proposition]   
> let $q=(a,b,c)$ be a  [BQF](#^ebdd1f)with $\text{disk}(q)=D\leq0$.
> Then for a given $n\in \mathbb{Z}$ there are at most a finite number of $x,y\in \mathbb{Z}$ such that $q(x,y)=n$

`\begin{proof}`
 say $q(x,y)=n$ then
$$
\begin{align}
4an & =(2ax+by)^{2}-Dy^{2} \\
 4an& \geq-Dy^{2} \\
 \frac{4an}{-D}& \geq y^{2} \\
\iff |y| & \leq \sqrt{ \frac{4an}{-D} } \\
\end{align}
$$
which show $y$ has finitely many values
also
$$
\begin{align}
(2ax+by)^{2} & \leq {4}an \\
\implies |2ax+by| & \leq \sqrt{ 4an }
\end{align}
$$
this show that for any value of $y$ there are finitely many values of $x$ $\implies$ there are finitely many values of $x,y$ 


`\end{proof}`



> [!remark ]  
> This is false for $D>0$ example $x^{2}-2y^{2}=1$

 Say $q(x,y)=n$ then
$4an=(2ax+by)^{2}-Dy^{2}\geq-Dy^{2}$

#23-sep 
# Equivalence
1. $Q(\mathbb{Z}^{2})=$ set of all [BQF](#^ebdd1f)
2. $M_{2}(\mathbb{Z})=$ set of all $2\times{2}$ Matrices
3. $GL_{2}(\mathbb{Z})=$ set of all $2\times{2}$ Invertable Matrices note the det here is 1 or -1
4. $SL_{2}(\mathbb{Z})=$ set of all $2\times{2}$ Matrices with determinant $1$ 
Note: $GL_{2}(\mathbb{Z})$ and $SL_{2}(\mathbb{Z})$ are both groups and $SL_{2}(\mathbb{Z})$ is the sub group of $GL_{2}(\mathbb{Z})$

let $q(x,y)=ax^{2}+bxy+cy^{2}\in Q(\mathbb{Z}^{2})$ and 
$$
\begin{align}
A=\begin{pmatrix}
	\alpha & \beta \\
	\gamma & \delta
\end{pmatrix} \in M_{2}(\mathbb{Z}) 
\end{align}
$$
Define the new [BQF](#^ebdd1f) $q.A$ by
$$
\begin{align}
(q.A) & =q\left[A\begin{pmatrix}
x  \\
y
\end{pmatrix}\right] \\
 & q(\alpha x+\beta y, x\gamma+\delta y)
\end{align}
$$
This is just a linear change of variable
$$
\begin{align}
(q.A)(x,y)=a(\alpha x+\beta y)^{2} +b(\alpha x+\beta y)(\gamma x+\delta y)+c(\gamma x+\delta y)^{2} 
\end{align}
$$

> [!proposition] 
> Let $q\in Q(\mathbb{Z}^{2})$ then
> 1. $q.I=q$
> 2. $(q\cdot A)\cdot B=q(A\cdot B)$ 

`\begin{proof}`
i) 
$$
\begin{align}
q\cdot I(x,y) & =q\left[I\begin{pmatrix}
x  \\
y
\end{pmatrix}\right] \\
 & =q\left[  
\begin{pmatrix}
1 & 0 \\
0 & 1 \\

\end{pmatrix}
\begin{pmatrix}
x  \\
y
\end{pmatrix}\right] \\
 & =q\begin{pmatrix}
x  \\
y
\end{pmatrix}
\end{align}

$$
ii) 
$$
\begin{align}
[(q\cdot A)\cdot B](x,y) & =(q\cdot A)\left[ B\begin{pmatrix}
x  \\
y
\end{pmatrix} \right]  \\
 & =(q\cdot A)\left[ \begin{pmatrix}
x'  \\
y'
\end{pmatrix} \right] \ \ \ \text{where } \begin{pmatrix}
x' \\
y'
\end{pmatrix}=\begin{pmatrix}
x  \\
y
\end{pmatrix} \\
 & =q\left[ A\begin{pmatrix}
x' \\
y'
\end{pmatrix} \right]  \\
 & =q\left[ AB\begin{pmatrix}
x \\
y
\end{pmatrix} \right]  \\ & =(q\cdot AB)\begin{pmatrix}
x \\
y
\end{pmatrix}   \\


\end{align}
$$


`\end{proof}`

---

>[!definition]  
> let $q_{1}$, $q_{2} \in Q(\mathbb{Z}^{2})$ 
> we say that $q_{1}$ is equivalent to $q_{2}$ if $\exists \ A \in GL_{2}(\mathbb{Z})$ st $q_{2}=q_{1}A$
> we say $q_{1}$ is properly equivalent to $q_{2}$ if $\exists \ A\in SL_{2}(\mathbb{Z})$ st $q_{2}=q_{1}\cdot A$ 
> Notation
> $q_{1}\sim q_{2}$ equivalent 
> $q_{1}\sim^{+} q_{2}$ properly equivalent 

> [!definition] mat of Binary Quadratic Form
$$\begin{align}\text{mat }q= \begin{pmatrix}2a & b\\b & 2c\end{pmatrix}\end{align}$$
$\det(\text{mat}q)=-\text{disc }(q)$


> [!exercise] 
> what is $\text{mat }(q\cdot A)$

Hint:
$$
\begin{align}
2q(x,y)=(x,y)\text{mat } q\begin{pmatrix}
x\\ y
\end{pmatrix}
\end{align}
$$
(question::why is there a 2)
let $q_{1}=q\cdot A$ 

$$
\begin{align}
2q_{1}(x,y)=(x,y)\text{mat }q_{1}\begin{pmatrix}x \\ y\end{pmatrix} 
\end{align}
$$
$$
\begin{align}
 \implies2(q\cdot A)(x,y) & =(x,y)\text{mat }(q\cdot A)\begin{pmatrix}x \\ y\end{pmatrix} \\
(x,y)\text{mat }(q\cdot A)\begin{pmatrix}x \\ y\end{pmatrix} & =2(q\cdot A)(x,y) \\
& =2q\left[ A  (x,y)^{T}   \right]\\
& =2q\left[   (x',y')^{T}   \right] \\
 & =(x',y')(\text{mat }q)\begin{pmatrix}x'\\ y' \end{pmatrix} \\
 & =\left( A \begin{pmatrix}x\\ y \end{pmatrix} \right) ^{t}(\text{mat }q)A\begin{pmatrix}x\\ y \end{pmatrix}   \\
(x,y)\text{mat }(q\cdot A)\begin{pmatrix}x \\ y\end{pmatrix}  & =(x,y)A^{T} (\text{mat }q)A\begin{pmatrix}x\\ y \end{pmatrix}  
\end{align}
$$

Hence $\text{mat }q.A=A^{T}\cdot\text{mat }q \cdot A$ 
> [!theorem] 
> let $q_{1}\sim q_{2}$
> 1. then $\text{disc }q_{1}=\text{disc }q_{2}$
> 2. $q_{1}$ and $q_{2}$ represents the same set of integers the same number of times
> 3. $q_{1}$  and $q_{2}$ are either both primitive or both non-primitive

^216a99


`\begin{proof}`
say $q_{2}=q_{1}A$ with $A\in GL_{2}(\mathbb{Z})$
$$
\begin{align}
\text{disc } q_{2 } & =-\det(\text{mat } q_{2})\\
\ & =-\det(A^{T}(\text{mat } q_{1})A )\\
\ & =-\det(A^{T})\det(\text{mat }q_{1})\det ( A )\\
\ & =-\det(A)^{2} \det(\text{mat }q_{1})\\
\ & =- \det(\text{mat }q_{1})=\text{disc } q_{1}
\end{align}
$$
ii) say $q_{2}(x,y)=n$
then 
$$
q_{1}\left[ A\begin{pmatrix}x \\ y\end{pmatrix} \right]=n
$$
if 
$$
\begin{align}
q_{1}(u,v) & =m \\
  \text{then,} &  \\
q_{2} & =\left( A^{-1}\begin{pmatrix}u \\ v\end{pmatrix}  \right) =m \\
  \text{also let,} & \\
q_{2}(x,y) & =n\\
q_{2}(x',y') & =n\\
\text{with } (x,y) & \neq(x',y') \\
\text{then} &  \\
q_{1}\left[ A\begin{pmatrix}x \\ y\end{pmatrix} \right]  & =n \\
q_{1}\left[ A\begin{pmatrix}x' \\ y'\end{pmatrix} \right] &  =n \\
\text{with } A\begin{pmatrix}x \\ y\end{pmatrix} & \neq A\begin{pmatrix}x' \\ y'\end{pmatrix}
\end{align}
$$

iii)
$$
\begin{align}
q_{1} & =(a,b,c) \ \ \text{primitives} \\
q_{2} & =(a',b',c') \\
q_{2} & =q_{1}\cdot A
\end{align}
$$
then $d$ divides $q_{2}(x,y) \forall \ x,y \in \mathbb{Z}$ 
since the set of the values of $q_{1}$ and $q_{2}$ are he same it follows that $d$ divides $q_{1}(x,y) \forall \ x,y \in \mathbb{Z}$ 
if $q_{1}$ is primitive then $d=1$ is the maximum value of $d$ which implies  $q_{2}$ is primitive
if $q_{1}$ is not primitive then $\exists \ d>1$ which implies $q_{2}$ is not primitive



> [!exercise] $\sim$ and $\sim^{+}$ are equivalence relations on $Q(\mathbb{Z}^{2})$ 


>[!theorem] 
>let $q\in Q(Z^{2})$ and $n\in \mathbb{Z}$ then $q$ represents $n$ properly iff
>$q\sim^{+}(n,b,c)$
>form some $b,c \in \mathbb{Z}$ 
>moreover if $n\neq{0}$ then  $\exists \ b$ such that $-|n|<|b|\leq|n|$

^6cf17c

`\begin{proof}`
suppose $q\sim^{+}(n,b,c)=q'$
say, $q'=qA, A\in SL_{2}(\mathbb{Z})$ 
$$
\begin{align}
A=\begin{pmatrix}
\alpha  & \beta\\ \gamma  & \delta
\end{pmatrix}
\end{align}
$$
then
$$
\begin{align}
q'(1,0)=n & =q\cdot A\begin{pmatrix}1\\ 0\end{pmatrix} \\
& =q\cdot A\begin{pmatrix}1\\ 0\end{pmatrix} \\
& =q(\alpha,\gamma)\\
\end{align}
$$
since $\alpha\delta-\beta\gamma=1$ $A\in SL_{2}(\mathbb{Z})$ is possible
so $q$ properly represent $n$
Now the other way 
assume $q$ properly represents $n$ say,
$$
\begin{align}
q(\alpha,\gamma)=n \text{ with } \gcd(\alpha,\gamma)=1
\end{align}
$$
we need to show that 
$$
\begin{align}
q\sim^{+}(n,b,c) \text{ for some } b,c \in \mathbb{Z}
\end{align}
$$
Now $\gcd(\alpha,\gamma)=1\implies$ we can find $\beta,\gamma \in Z$ such that $\alpha\delta-\beta\gamma=1$ [[bezout's theorem]] 
let 
$$
\begin{align}
A=
\begin{pmatrix}
	\alpha & \beta \\
	\gamma & \delta
\end{pmatrix} \\
q'=q*A
\end{align}
$$
Note that 
$$
\begin{align}
q'(1,0) & =(qA)\begin{pmatrix}1 \\ 0\end{pmatrix} \\
& =q(\alpha,\gamma) \\
& =n  \\
\implies q' & =(n,b,c)
\end{align}
$$
for some $b,c\in \mathbb{Z}$ this proves the first part

let $n\neq{0}$ we can write 
$$
\begin{align}
b=2|n|u + r
\end{align}

$$
with $-|n|<r\leq|n|$
let $q''=q'B$ where (question::is this correct how to prove it) 
$$
\begin{align}
B=\begin{pmatrix}
1 & -u  \\
0 & 1
\end{pmatrix}
\end{align}
$$


> [!remark] principle forms of disc 
> $D$ can be $1,0 \pmod{4}$ and they can be simply represented by
> $x^{2}-\frac{D}{4}y^{2}$ if $0\pmod{4}$
> $x^{2}+xy+\frac{1-D}{4}y^{2}$ if $1\pmod{4}$
> these are known as principal forms of disc $D$ 

> [!theorem] Lagrange
> Let $D,n\in \mathbb{Z}$. The following are equivalent 
> 1. $D$ is a square $\pmod{4n}$
> 2. there is a [BQF](#^ebdd1f)  $q$ of discriminant $D$ which properly represents $n$ 

^f95cab

1$\implies$ 2
say $b^{2}=D+4nc$ for some $c\in \mathbb{Z}$ $\implies b^{2}-4nc=D$
let $q=(n,b,c)$ then $q(1,0)=n$ so $q$ properly represents $n$ 
2 $\implies$ 1
let $q$ be a [BQF](#^ebdd1f) of disc $D$ which properly represents $n$ then by [[3. Binary#^6cf17c]] 
$$
\begin{align}
q\sim^{+}(n,b,c) 
\end{align}
$$
for some $b,c\in \mathbb{Z}$ [[#^216a99]] 
since $D=\text{disc }q=\text{disc }(n,b,c)=b^{2}-4nc$ 
we get 
$$
\begin{align}
b^{2} \equiv D \pmod{4n}
\end{align}
$$
hence $D$ is a square mod $4n$ 
#26-sep 

---
> [!corollary]   
> let $D\equiv 1,0 \pmod{4}$ let $p$ be a prime such that  $\left( \frac{D}{p} \right)=1$ Then there is a [BQF](#^ebdd1f) $q$ of the disc $D$ which properly represents $p$ . This form is unique up to equivalence

 `\begin{proof}`
 We know that $q$ represents $p$ from [[#^f95cab]]  
 By Lagrange, there is a bqf $q$ which properly represents $p$. Then we know that  ^7902f4
 $$
\begin{align}
q \sim^{+} (p,b,c)
\end{align}
$$
for some $b,c\in \mathbb{Z}$ with $-p<b\leq p$ Now $\begin{bmatrix}-1 & 0 \\ 0 & 1\end{bmatrix}$ converts $(p,b,c)\to(p,-b,c)$ 
so we may chose $0\leq b\leq p$ thus 
$$
\begin{align}
q \sim (p,b,c)
\end{align}
$$
with $0\leq b\leq p$ so let $q'$ be another form of disc $D$ which properly represents $p$.
As above we may take 
$$
\begin{align}
q'\sim(p,b',c')
\end{align}
$$
with $0\leq b'\leq p$ 
we need to prove that $b=b',c=c'$ 
since $(p,b,c)\text{ and } (p,b',c')$ have the same discriminant we have
$$
\begin{align}
b^{2} -4pc & =b'^{2} -4pc' \\
\implies (b+b')(b-b') & =0\pmod{4p}\\ 
	\implies \text{2 divides both }  & b+b' \text{and} b'-b   \\


\end{align}
$$
 (todo::why cant 4 divide one of it and the other be odd) 




if $p|b-b'$ then we are done $\implies b=b'$ $\because$ $b$ and $b'$  $\leq p$ 
so suppose $p \nmid b-b'$ but $p|b+b'$ 
$$
\begin{align}
\implies b+b'=2p \text{ or }0 \because b,b'\leq p\\
b=b'=p \text{ or } 0
\end{align}
$$

so in any case $b=b'$
it follows that $c=c'$
## Binary Quadratic Forms with given Discriminant
An integer $D\in \mathbb{Z}$ is called a discriminant if it is the discriminant of some BQF 
recall that $D$ is a discriminant $\iff D\equiv0\text{ or } 1\pmod{4}$ 

> [!definition] Fundamental Discriminant
We say that a discriminant $D$ is a Fundamental Discriminant if every bqf of discriminant $D$ is primitive

# Example
$5$ is a fundamental discriminant for if $q=(a,b,c)$ is of discriminant $5$ and if $d=\gcd(a,b,c)$ then $d ^{2}| b^{2}-4ac=5$ which implies $d=1$.
$4$ is a fundamental discriminant.
$8$ is a fundamental discriminant.
as if $d^{2}|\text{disc }q=8$ then $d$ can be $1,2$ if $d$ is $2$.
$(2a',2b',2c')$ has a disc of $8=4b'^{2}+a'c'4\implies{2}=b'^{2}+a'c'$ we can we the second equation is also a discriminant hence it cant be equal to $2$.

> [!proposition] 
> let $D$ be a discriminant. Then $D$ is a fundamental discriminant if
> i) $d\equiv1\pmod{4}$ and $D$ is square free
> ii) $d\equiv{0}\pmod{4}$ and $\frac{d}{4}$ is square free and $\frac{D}{4}\equiv{2}\text{ or }3 \pmod{4}$


`\begin{proof}`
Let $D$ be a fundamental discriminant 

Case I: $D\equiv1\pmod{4}$
we claim that $D$ is square free suppose 
$$
\begin{align}
D=r^{2} s
\end{align}
$$
with $s$ square free if $r\neq1$ then 
$$
\begin{align}
rx^{2} +rxy+\frac{r(1-s)}{4}y^{2} 
\end{align}
$$
note that: $r^{2}s=D\equiv{1}\pmod{4}\implies r^{2}\equiv s\equiv \pmod{4}$
but then the above bqf is not primitive hence $D$ should be square free
Case II: $D\equiv{0}\pmod{4}$

If $\frac{D}{4}\equiv{0}\pmod{4}$ 
$$2x^{2}-\frac{D}{8}y^{2}$$ is not primitive so $\frac{D}{4}$ can be congruent to 4

suppose $\frac{d}{4}\equiv1 \pmod{4}$ 

$$2x^{2} +2xy+\frac{4-D}{8}y^{2} $$ is a bqf which is not primitive 

then we are left with 
$$\frac{D}{4}\equiv2 \text{ or } 3\pmod{4} $$
Finally we prove that $\frac{D}{4}$is square free 

$$
\begin{gather}
\frac{D}{4}  =r^{2} s \\
\text{then }  rx^{2} -rsy^{2} \text{ is a not primitive }
\end{gather}
$$
---------------------------------------------------------------------------------
#27-sep
> [!exercise] 
> What are all the bqf of disc 0?


Suppose  $q \in Q(\mathbb{Z}^{2})$ has disc 0, say $q=(a,b,c)$

case I: $a=0$ 
then $\text{disc }q=D=b^{2}+4\cdot0\cdot c\implies b=0$
hence $q=(0,0,c)$
case II:  $A\neq0$ 
then 
$$
\begin{align}
4aq(x,y) & =(2ax+by)^{2}  \\
\implies q(-b,2a) & =0 \text{ with } (-b,2a)\neq(0,0) \\
\implies q \text{ properly represents } 0
\end{align}
$$
there fore 
$$
\begin{align}
	q & \sim^{+} (0,b,c) 
\end{align}
$$
for some $b,c\in \mathbb{Z}$ again $b^{2}=0\implies b=0$
$$
\begin{align}
\therefore q \sim^{+} (0,0,c) 
\end{align}
$$
suppose $c\neq c'$

now let 
$$
\begin{align}
	q & =(0,0,c) \\
 q' & =(0,0,c')
\end{align}
$$
is $q'\sim^{}q$ (NO!)
as $q=\left\{ cy^{2} \right\}$
and $q'=\left\{ c'y^{2} \right\}$ 
hence if $c'\neq c$ $q$ and $q'$ are complete different.
hence there are infinitely many bqf of discriminant 0 which are in equivalent 

> [!proposition] 
> Let $D=d^{2}\neq0$  with $d>0$. Then up to proper equivalence there are only finitely many distinct  bqf of discriminant  $D$  

`\begin{proof}`
Let $q$ be of $\text{disc }D=d^{2}\neq0$ hence $q$ properly represents $0$ and hence 

$$
\begin{align}
q  & \sim^{+} (0,b,c) \text{ for some } b,c \in \mathbb{Z}  \\
\text{then } b^{2}  & =D=d^{2}  \\
	\implies b & =\pm d\neq0
\end{align}
$$
write $c=bu+r$ with $0\leq r\leq|b| \ u,r\in \mathbb{Z}$ then
$$
\begin{align}
	(0,b,c)  \underbrace{ \sim^{+}  }_{ \begin{bmatrix}1 & -u \\ 0 & 1\end{bmatrix}  }  & (0,b,c-bu) \\
 = & (0,b,r)
\end{align}
$$
so there are at most $|b|=d$ distinct form up to proper equivalence

`\end{proof}`

> [!lemma] Lagrange Reduction
> Let $D\in \mathbb{Z}$ be a discriminant $D\neq{0}$ and not a square 
> Then, $q$ is properly equivalent to a form (a, $b$ ,c) with $|b|\leq|a|\leq|c|$ 
> also, such a form $(a,b,c)$ satisfying $1\leq|a|\leq \sqrt{ \frac{|D|}{3} }$ 

`\begin{proof}`

Let,
$$
\begin{align}
V=\left\{  |q(x,y)|;\text{s.t} \gcd(x,y)=1\right\}
\end{align}
$$
Since $D$ is not a square, $0\notin V$ let $a=q(x,y)$ be such that $|a|=\min V$.
Since $q$ represents a, we have from [[#^6cf17c]].
$$
\begin{align}
&q \sim^{+} (a,b,c) \text{ for some } (a,b,c) \text{ with } -|a|<b\leq |a| \\
&\implies |b|\leq|a| \text{ since  $q$  also repsents c we have   }\\
&\implies |a|\leq |c| \text{ then } \\
&\implies |b|\leq|a|\leq|c| \text{ now why is } a<c

\end{align}
$$
$$
\begin{align}
	 b^{2} -4ac & =D \\
\implies |D| & \geq 4|ac| -|b|^{2}  \\
 & \geq 4|a|^{2} -|a|^{2} \\
 & =3|a|^{2} \\
\implies 1\leq &|a| \leq \sqrt{ \frac{|D|}{3} }
\end{align}
$$


`\end{proof}`

> [!theorem]  Lagrange
> Let $D\in \mathbb{Z}$ be a discriminant $D\neq0$ and $D$ not a square then up to proper equivalence only finite many distinct bqf of discriminant D 

`\begin{proof}`
we know 
$q \sim^{+}(a,b,c)$ with $(|b|\leq|a|\leq|c|)$

$$
\begin{gather}
1\leq|a|\leq \sqrt{ \frac{|D|}{3} }
\end{gather}
$$
hence there are only finitely many possibilities for $a$ and hence for $b$ and $|b|\leq|a|$ since
$$
\begin{align}
b^{2} -4ac=D
\end{align}
$$
the possibilities for $c$ is also finite 
`\end{proof}`

> [!definition] 
> let $D\neq0$ be a discriminant 
> $\mathcal{Cl}(D) =$ set of proper equivalence classes of bqf of $\text{disc }D$ 
> $\mathcal{P}(D) =$ set of proper equivalence classes of primitive bqf of disc  $D$   
> we have $b(D)=|\mathcal{P}(D)|$(Disc of P ) this is know as the Class Number of  $D$  

## Example 
1. What is $h(-4)$ 
Since $D=-4<0$ we assume $a>0$ 
then note that $4ac=b^{2}+|D|>0$ 
than $|b|\leq a\leq c$
since 
$$
\begin{align}
b^{2}  & \equiv D \pmod{4} \\
\implies b & \equiv0\pmod{2}   \\
\text{and } |b|\leq a\leq \sqrt{ \frac{4}{3} }<2
\end{align}
$$
thus the only possibility is $b=0$ hence $(a,b,c)=(a,0,c)$. 
Also $a=1$ then
$$
\begin{align}
a \sim^{+}(1,0,c) 
\end{align}
$$
since $-4c=-4$ we have $c=1$ then
$$
\begin{align}
q \sim^{+} (1,0,1)
\end{align}
$$
also recall that if $\left( \frac{D}{p} \right)=1$ $q$ primitively represents p
 $i$ .$e$ , if $\left( -\frac{4}{p} \right)=1$, then there exist $x,y\in \mathbb{Z}$ such that $x^{2}+y^{2}=p$
 Now, $\left( -\frac{4}{p} \right)=\left( \frac{-1}{p} \right)=\left( -1 \right)^{\frac{p-1}{2}}=1\iff p\equiv{1}\pmod{4}$  
 Then every prime $p$ can be written as a sum of square.

> [!theorem] 
> let $D\in \left\{ -3,-4,-7,-8,-11,-12,-19,-16,-27,-28,-43,-67,-163 \right\}$ then $h(D)=1$ 
> Gauss conjecture that $h(D)\neq1$ for any other $D<0$ 


> [!conjecture] UNSOLVED
> Are there infinitely many $D>0$ $s$.$t$. $h(D)=1$ 
> 

`\begin{proof}`
`\end{proof}`