
> [!definition] Multiplicative Function
> An [[4. Arithmetic Functions#^919b57|Arithmetic Function]] $f$ is called multiplicative if $f\neq0$ and $f(mn)=f(m)f(n) \forall \ \gcd(m,n)=1$

^550189

> [!remark] 
> If $f$ is multiplicative then $f(1)=1$

 >[!definition] Completely Multiplicative Function
> An [[4. Arithmetic Functions#^919b57|Arithmetic Function]] $f$ is called Completely multiplicative if $f(mn)=f(m)f(n) \forall m,n \in \ZZ$ 

## Examples
$I,\mathbb{1},\tau,u,\varphi,\mu$ are [[#^550189|Multiplicative]] 

$\Lambda,\omega,\Omega$ are non-multiplicative
> [!theorem] 
>Prove $\tau=\left\{ \text{\# of divisors} \right\}$ is [[#^550189|Multiplicative]] 


`\begin{proof}`
lets show there is a bijection 
$$
\begin{align}
F:\tau(m)\times \tau(n) & \to \tau(mn) \\
\implies (a,b) & \mapsto ab
\end{align}
$$
let $d\in \tau(mn)$ we want to find $(a,b)\in \tau(m)\times \tau(n)$ $s$ . $t$ .
$$
\begin{align}
ab=d
\end{align}
$$
let 
$$
\begin{align}
	a & =(d,m) \\
	b & =(d,n) \\
	\implies a\times b & =(d,mn)
\end{align}
$$
Hence $d=ab$ 
this prove $F$ is surjective 
now lets prove $F$ is injective 

$$
\begin{align}
F(a,b) & =F(a',b') \text{(say)} \\
\implies ab & =a'b' \\
\implies a & =a' \text{ as } \gcd(a,b')=1 \\
\text{ similarly } b & = b'
\end{align}
$$
hence $F$ is bijection 
`\end{proof}`

> [!proposition] 
> If $f$ and $g$ are multiplicative then so is $f * g$. conversly if $f$ and $f*g$ is multiplicative the $g$ is multiplicative 

`\begin{proof}`
Write $h=f*g$
let $(m,n)=1$ we want to show that 
$$
\begin{align}
h(mn) & =h(m)h(n) \\
h(mn) & =\sum_{d|mn}f(d)g\left( \frac{mn}{d} \right)\\
h(mn) & =\sum_{a|m \text{ and } b|n}f(ab)g\left( \frac{mn}{ab} \right)\\
h(mn) & =\sum_{a|m \text{ and } b|n}f(a)g\left( \frac{mn}{a} \right)f(b)g\left( \frac{mn}{b} \right)\\ 
h(mn) & =\sum_{a|m}f(a)g\left( \frac{mn}{a} \right)\sum_{b|m}f(b)g\left( \frac{mn}{b} \right)\\ 
h(mn) & =h(m)h(n)\\
\end{align}
$$
we have proved the first part now the second part 

suppose $g$ is not multiplicative 
then there $\exists \ \gcd(m,n)=1$ $s$ . $t$ . 
$$
\begin{align}
g(mn)\neq g(m)g(n)
\end{align}
$$
chose such $m$ , $n$ so that $mn$ is the smallest possible 

Case I suppose $mn=1$ 
then $m=n=1$
now 
$$
\begin{align}
h(mn) & =h(1)=f(1)g(1) \\
 & = q(1)\neq1
\end{align}
$$
then $h$ is not multiplicative 
So $mn>1$ 
now 
$$
\begin{align}
h(mn) & =\sum_{d|mn}^{} f(a)g\left( \frac{mn}{d} \right)\\
h(mn) & =g(mn)+\sum_{d|mn,d>1}^{} f(a)g\left( \frac{mn}{d} \right)\\
h(mn) & =g(mn)+\sum_{a|m,\ b|n, \ ab>1}^{} f(ab)g\left( \frac{m}{a} \frac{n}{b} \right)\\
h(mn) & =g(mn)+\sum_{a|m,\ b|n, }^{} f(a)f(b)g\left( \frac{m}{a} \right)g\left( \frac{n}{b} \right)\\
h(mn) & =g(mn)+\sum_{a|m,\ b|n, \ ab>1}^{} f(a)f(b)g\left( \frac{m}{a} \right)g\left( \frac{n}{b} \right) - g(m)g(n)\\
h(mn) & =g(mn)+h(m)h(n) - g(m)g(n)\\
\end{align}
$$
as $g(mn)-g(m)g(n)$ is not 0 then $h(mn)$ is not multiplicative

$$
\begin{align}
I(n)=\begin{cases}
1 \text{ if } n=1 \\
0 \text{ otherwise}
\end{cases}
\end{align}
$$
> [!corollary] 
> Let $f$ and $g\in \mathcal{A}$ such that $f*g=I$ then $f$ is multiplicative $\iff$ $g$ is multiplicative

> [!proposition] 
 Let $f$ and $g\in \mathcal{A}$ then $f^{-1}$ exist if $f(1)=0$
> 

`\begin{proof}`

Suppose $f^{-1}$ exist then 
$$
\begin{align}
f*f^{-1} (1) & =1 \\
\implies f(1)f(1) & =1 \\
\implies f(1) & \neq0
\end{align}
$$
conversely suppose $f(1)\neq0$ 
suppose $f^{-1} \exists$ then we must have
$$
\begin{align}
(f*f^{-1} )(1) & =1 \\
\implies f^{-1} & =\frac{1}{f(1)} \text{ which is defined as } f(1)\neq0
\end{align}
$$

Lets solve it by induction 

Suppose $f^{-1}(1)\dots f^{-1}(n)$ is defined 
we want to define $f^{-1}(n+1)$ now we need 
such that 

$$
\begin{align}
f*f^{-1}(n+1) & =0 \\
\implies 0 & = \sum_{d|n+1}f(d)f^{-1}\left( \frac{n+1}{d} \right) \\
\implies 0 & =f^{-1}(n+1)f(1)+ \sum_{d|n+1,d>1}f(d)f^{-1}\left( \frac{n+1}{d} \right) \\
\implies f^{-1}(n+1) & =\frac{1}{f(1)}\sum_{1<d|n+1} f(d)f^{-1}\left( \frac{n+1}{d} \right) 
\end{align}
$$
this completes the proof
`\end{proof}` 

## Examples 

1. $\mu*u=I$
2. find $\mu^{-1}$
as $\mu$ is multiplicative so is $\mu^{-1}$ so its sufficient to find $\mu^{-1}(p^{k})$ for all primes and $n$ $\in \ZZ^{+}$

$$
\begin{align}
\varphi^{-1} (p) & =1-p\\
\varphi^{-1} (p^{2} ) & =1-p\\
\varphi^{-1} (p^{3}) & =1-p \\
\vdots & \qquad \vdots \\
\varphi^{-1} (p^{n}) & =1-p \\
\text{hence } \varphi^{-1}(n) & =\prod_{p|n}(1-p)
\end{align}
$$


> [!remark] 
> If $h=f*g$ then 
$$
\begin{align}
					\sum_{n=1}^{\infty} \frac{h(n)}{n^{s} }=\sum_{m=1}^{\infty} \frac{f(m)}{m^{s} }\sum_{n=1}^{\infty} \frac{g(n)}{n^{s} }
\end{align}
$$

proof

$$
\begin{align}
\sum_{m=1}^{\infty} \frac{f(m)}{m^{s} }\sum_{n=1}^{\infty} \frac{g(n)}{n^{s}} & = \left( \frac{f(1)}{1^{^{2} } }+\frac{f(2)}{2^{s} }\dots \frac{f(m)}{m^{s} }\dots \right) \left( \frac{g(1)}{1^{^{2} } }+\frac{g(2)}{2^{s} }\dots \frac{g(n)}{n^{s} }\dots \right) \\
 & = \frac{f(1)g(1)}{1^{s} } + \frac{f(2)g(1)\dots+f(1)f(2)}{2^{s} }+\dots+\frac{f(n)g(1)\dots+f(1)f(n)}{n^{s} } \\
		 & = \sum_{n=1}^{\infty} \frac{(f*g)(n)}{n^{s} }=\sum_{n=1}^{\infty} \frac{h(n)}{n^{s} }
\end{align}
$$


