Let $k\in \ZZ^{+}$ a complex sequence $(u_{n})_{n\geq0}$ is said to be satisfy a Linear reccurrence of order $k$ if there are fixed complex numbers $b_{1},\dots b_{k}\st$ 
$$
\begin{align}
		u_{n+k}  & = b_{1}u_{n}+\dots b_{k} y_{n+k}  \forall n\geq0
\end{align}
$$

## Example 
$F_{n}$ a Fibonacci sequence defined by $F_{0}=0,F_{1}=1$
satisfies a LR of order 2


*We will be mostly interested in k=2* 
then $u_{n}=au_{n-1}+bu_{n-2}  \to *$  ^8a8953

for all $n\geq2$

Let $u_{n}$ be a sequence satisfying [[#^8a8953|*]] 
consider

$$
\begin{align}
		f(z) & =\sum_{n=0}^{\infty} u_{n} z^{n} \\
\text{let} Q(z) & =1-az-bz^{2}  \\
	P(z)  & = f(z)Q(z) \\
 & =(u_{o}+u_{1}z +u_{2}z^{2} \dots)(1-az-bz^{2} ) \\
 & = u_{0}+(u_{1}-au_{0})z+(u_{2}-au_{1}-bu_{0})z^{2} +\dots \\
 & = u_{0}+(u_{1}-au_{0} )z 
\end{align}
$$
thus 
$$
\begin{align}
f(z)= \frac{P(z)}{Q(z)}
\end{align}
$$

Let $D(a,b)$ denote the set of all complex sequence $(u_{n})$ satisfying
$$
\begin{align}
u_{n}=au_{n-1}+bu_{n-2} \forall n\geq2   
\end{align}
$$
clearly if $(u_{n})(v_{n})\in(a,b)$
then 
$$
\begin{align}
			\alpha(u_{n} )+\beta(v_{n} )\in d(a,b) 
\end{align}
$$
where 
$$
\begin{align}
	\alpha(u_{n} )=(\alpha u_{0},\alpha u_{1},\dots ) \\
\text{and} \\
(u_{n} )+v_{n}=(u_{n}+v_{n}  ) 
\end{align}
$$
then $D(a,b)$ is vector space over $\CC$ 
since $u_{0}$ and $u_{1}$ completely determine it then it follows that $\dim D(a,b)=2$

let 

$$
\begin{align}
1-az-bz^{2} =(1-\lambda_{1}z )(1-\lambda_{2}z )
\end{align}
$$
then 
$$
\begin{align}
Q\left( \frac{1}{\lambda_{1} } \right) & =Q\left( \frac{1}{\lambda_{2} } \right)=0 \\
\lambda_{1}+\lambda_{2} & =a  \\
  \lambda_{1}\lambda_{2}=-b  
\end{align}
$$
also
$$
\begin{align}
1-\left( \frac{a}{\lambda_{i} } \right)- \left( \frac{b}{\lambda_{i}  }\right) & =  0\\
\lambda_{i}^{n}   & =a\lambda_{i}^{n-1}+  \beta\lambda_{i} ^{n-2} 
\end{align}
$$
Hence $\lambda_{1}^{n}$ and $\lambda^{n}_{2}$

Satisfying the recurrence relation 

$$
\begin{align}
u_{n}=au_{n-1}+bu_{n-2}   
\end{align}
$$
chose a and $b$ such that $\lambda_{1}\neq\lambda_{2}$ then 
$(\lambda_{1},\lambda_{2})\in D(a,b)$ are distinct 

> [!claim] 
> $\lambda_{1}^{n}$ and $\lambda_{2}^{n}$ are linearly independent 

if dependent $\lambda_{1}^{0}=\alpha\lambda_{2}^{0}\implies\alpha=0\implies\lambda_{1}=\lambda_{2}\implies\impliedby$ the fact they are distinct 

## Example 

1. Fib series
$Q(z)=1-z-z^{2}$ 
the roots are $\frac{\sqrt{ 5 }+1}{2}, \frac{-\sqrt{ 5 }+1}{2}$
then we can find  $\alpha,\beta \st$ 

$$
\begin{align}
F_{n} & =\alpha\lambda_{1}^{n_{0}}+\beta\lambda_{2}^{n} \\
\text{Now, }     F_{o} & =0 \implies \alpha+\beta
=0 \\
F_{1} & =1\implies \alpha\lambda_{1}+\beta \lambda_{2}=1  \end{align}
$$
suppose
$$
\begin{align}
1-az-az^{2}  & =(1-\lambda z)^{2}  \\
\implies 2\lambda & =a \\
 \implies \lambda^{2} &  =-b
\end{align}
$$
the discriminant is 
$$
\begin{align}
a^{2} +4b=0
\end{align}
$$
then
$$
\begin{align}
2\lambda^{n}=a\lambda^{n-1}  
\end{align}
$$
> [!claim] 
> $(n\lambda)^{2}\in D(a,b)$
and 
$\lambda^{n}, n\lambda^{n}$ form a basis of $D(a,b)$ 

`\begin{proof}` 

we have 

$$
\begin{align}
\lambda^{2} -a\lambda+b
\end{align}
$$
as $\frac{1}{\lambda}$ is a root of $1-az-bz^{2}$

then 
$$
\begin{align}
\left(n-2\right) \lambda^{n} & =(n-2)a\lambda^{n-1}  + b(n-2)\lambda^{n-2}  \\
 \implies n\lambda^{n} & =2\lambda^{n}+(n-2)a\lambda^{n-1}   +b(n-2)\lambda^{n_{0}1}  \\
 & = a\lambda^{n-1} +  (n-2) a \lambda^{n-1} + b(n-2)\lambda^{n-2}  \\
 & = a(n-1)\Lambda^{n-1} + b(n-2) \lambda^{n-2 }  
\end{align}
$$
so $(n\lambda^{n})\in D(a,b)$
also $\lambda^{n} and (n\lambda)^{n}$ are linearly independent
for if they were linearly independent then we would have 

$$
\begin{align}
\lambda^{n}=\alpha (n\lambda^{n} )
\end{align}
$$
for some $\alpha \in D$ 

ie, 
$$
\begin{align}
\lambda^{n} =\alpha n\lambda^{n} \forall n  
\end{align}
$$
for $n=1$ 

$$
\begin{align}
\lambda=\alpha\lambda\implies\alpha=1
\end{align}
$$
hence 

$$
		\begin{align}\lambda^{n} =n\lambda^{n} \forall n\geq0

\end{align}
$$
 `\end{proof}`